Foundation/Modal/Kripke/Hilbert/KT.lean
@@ -9,6 +9,12 @@ abbrev Kripke.ReflexiveFrameClass : FrameClass := { F | Reflexive F }
 
 namespace Hilbert.KT
 
+instance Kripke.sound : Sound (Hilbert.KT) (Kripke.ReflexiveFrameClass) := by
+  convert Hilbert.Geach.Kripke.sound (G := {⟨0, 0, 1, 0⟩});
+  . exact eq_Geach;
+  . unfold ReflexiveFrameClass MultiGeacheanConfluentFrameClass MultiGeachean;
+    simp [Geachean.reflexive_def];
+
 instance Kripke.consistent : System.Consistent (Hilbert.KT) := by
   convert Hilbert.Geach.Kripke.Consistent (G := {⟨0, 0, 1, 0⟩});
   exact eq_Geach;
