Foundation/Modal/Logic/WellKnown.lean
@@ -1,5 +1,14 @@
+import Foundation.Modal.Hilbert.Maximal.Unprovability
+import Foundation.Modal.Kripke.Hilbert.GL.Completeness
+import Foundation.Modal.Kripke.Hilbert.Grz.Completeness
+import Foundation.Modal.Kripke.Hilbert.K4
+import Foundation.Modal.Kripke.Hilbert.KD
+import Foundation.Modal.Kripke.Hilbert.S4
+import Foundation.Modal.Kripke.Hilbert.S5
+import Foundation.Modal.Kripke.Hilbert.Triv
+import Foundation.Modal.Kripke.Hilbert.Ver
 import Foundation.Modal.Logic.Basic
-import Foundation.Modal.Hilbert.WellKnown
+import Foundation.Modal.System.KT
 
 namespace LO.Modal
 
@@ -7,17 +16,233 @@ namespace Logic
 
 protected abbrev K4 : Logic := Hilbert.K4.logic
 
+instance : (Logic.K4).Normal := Hilbert.normal
+
+lemma K4.eq_TransitiveKripkeFrameClass_Logic : Logic.K4 = Kripke.TransitiveFrameClass.logic
+  := eq_Hilbert_Logic_KripkeFrameClass_Logic
+
+
+protected abbrev KD : Logic := Hilbert.KD.logic
+
+instance : (Logic.KD).Normal := Hilbert.normal
+
+lemma KD.eq_SerialKripkeFrameClass_Logic : Logic.KD = Kripke.SerialFrameClass.logic
+  := eq_Hilbert_Logic_KripkeFrameClass_Logic
+
+
+
+protected abbrev KT : Logic := Hilbert.KT.logic
+
+instance : (Logic.KT).Normal := Hilbert.normal
+
+lemma KT.eq_TransitiveKripkeFrameClass_Logic : Logic.KT = Kripke.ReflexiveFrameClass.logic
+  := eq_Hilbert_Logic_KripkeFrameClass_Logic
+
+
 protected abbrev S4 : Logic := Hilbert.S4.logic
+
 instance : (Logic.S4).Normal := Hilbert.normal
 
+lemma S4.eq_ReflexiveTransitiveKripkeFrameClass_Logic : Logic.S4 = Kripke.ReflexiveTransitiveFrameClass.logic
+  := eq_Hilbert_Logic_KripkeFrameClass_Logic
+
+
 protected abbrev S5 : Logic := Hilbert.S5.logic
+
 instance : (Logic.S5).Normal := Hilbert.normal
 
+lemma S5.eq_ReflexiveEuclideanKripkeFrameClass_Logic : Logic.S5 = Kripke.ReflexiveEuclideanFrameClass.logic
+  := eq_Hilbert_Logic_KripkeFrameClass_Logic
+
+
 protected abbrev GL : Logic := Hilbert.GL.logic
+
 instance : (Logic.GL).Normal := Hilbert.normal
 
+lemma GL.eq_TransitiveIrreflexiveFiniteKripkeFrameClass_Logic : Logic.GL = Kripke.TransitiveIrreflexiveFiniteFrameClass.logic
+  := eq_Hilbert_Logic_KripkeFiniteFrameClass_Logic
+
+
 protected abbrev Grz : Logic := Hilbert.Grz.logic
+
 instance : (Logic.Grz).Normal := Hilbert.normal
+
+lemma Grz.eq_ReflexiveTransitiveAntiSymmetricFiniteKripkeFrameClass_Logic : Logic.Grz = Kripke.ReflexiveTransitiveAntiSymmetricFiniteFrameClass.logic
+  := eq_Hilbert_Logic_KripkeFiniteFrameClass_Logic
+
+
+protected abbrev Triv : Logic := Hilbert.Triv.logic
+
+instance : (Logic.Triv).Normal := Hilbert.normal
+
+lemma Triv.eq_EqualityKripkeFrameClass_Logic : Logic.Triv = Kripke.EqualityFrameClass.logic
+  := eq_Hilbert_Logic_KripkeFrameClass_Logic
+
+
+protected abbrev Ver : Logic := Hilbert.Ver.logic
+
+instance : (Logic.Ver).Normal := Hilbert.normal
+
+lemma Ver.eq_IsolatedFrameClass_Logic : Logic.Ver = Kripke.IsolatedFrameClass.logic
+  := eq_Hilbert_Logic_KripkeFrameClass_Logic
+
+
+end Logic
+
+
+
+namespace Logic
+
+open Formula
+open System
+open Kripke
+
+theorem K_ssubset_KD : (Logic.K) ⊂ (Logic.KD) := by
+  constructor;
+  . exact Hilbert.weakerThan_of_dominate_axioms $ by simp [axiomK!];
+  . suffices ∃ φ, Hilbert.KD ⊢! φ ∧ ¬AllFrameClass ⊧ φ by simpa [K.eq_AllKripkeFrameClass_Logic];
+    use (Axioms.D (.atom 0));
+    constructor;
+    . exact axiomD!;
+    . apply Formula.Kripke.ValidOnFrameClass.not_of_exists_model_world;
+      let M : Model := ⟨⟨Fin 1, λ x y => False⟩, λ w _ => False⟩;
+      use M, 0;
+      constructor;
+      . tauto;
+      . simp [Semantics.Realize, Satisfies];
+
+theorem KD_ssubset_KT : (Logic.KD) ⊂ (Logic.KT) := by
+  constructor;
+  . exact Hilbert.weakerThan_of_dominate_axioms $ by simp [axiomK!, axiomD!];
+  . suffices ∃ φ, Hilbert.KT ⊢! φ ∧ ¬SerialFrameClass ⊧ φ by simpa [KD.eq_SerialKripkeFrameClass_Logic];
+    use (Axioms.T (.atom 0));
+    constructor;
+    . exact axiomT!;
+    . apply Formula.Kripke.ValidOnFrameClass.not_of_exists_model_world;
+      use ⟨⟨Fin 2, λ x y => y = 1⟩, λ w _ => w = 1⟩, 0;
+      constructor;
+      . tauto;
+      . simp [Semantics.Realize, Satisfies];
+
+theorem K_ssubset_KT : (Logic.K) ⊂ (Logic.KT) := by
+  trans;
+  . exact K_ssubset_KD;
+  . exact KD_ssubset_KT;
+
+theorem K_ssubset_K4 : (Logic.K) ⊂ (Logic.K4) := by
+  constructor;
+  . exact Hilbert.weakerThan_of_dominate_axioms $ by simp [axiomK!];
+  . suffices ∃ φ, Hilbert.K4 ⊢! φ ∧ ¬AllFrameClass ⊧ φ by simpa [K.eq_AllKripkeFrameClass_Logic];
+    use (Axioms.Four (.atom 0));
+    constructor;
+    . exact axiomFour!;
+    . apply Formula.Kripke.ValidOnFrameClass.not_of_exists_model_world;
+      let M : Model := ⟨⟨Fin 2, λ x y => x ≠ y⟩, λ w _ => w = 1⟩;
+      use M, 0;
+      constructor
+      . tauto;
+      . suffices (∀ (y : M.World), (0 : M.World) ≺ y → y = 1) ∧ ∃ x, (0 : M.World) ≺ x ∧ ∃ y, x ≺ y ∧ y ≠ 1 by
+          simpa [Semantics.Realize, Satisfies];
+        constructor;
+        . intro x;
+          match x with
+          | 0 => tauto;
+          | 1 => tauto;
+        . use 1;
+          constructor;
+          . omega;
+          . use 0;
+            constructor;
+            . omega;
+            . trivial;
+
+theorem KT_ssubset_S4 : (Logic.KT) ⊂ (Logic.S4) := by
+  constructor;
+  . exact Hilbert.weakerThan_of_dominate_axioms $ by simp [axiomK!, axiomT!];
+  . suffices ∃ φ, Hilbert.S4 ⊢! φ ∧ ¬ReflexiveFrameClass ⊧ φ by simpa [KT.eq_TransitiveKripkeFrameClass_Logic];
+    use Axioms.Four (.atom 0);
+    constructor;
+    . exact axiomFour!;
+    . apply Formula.Kripke.ValidOnFrameClass.not_of_exists_model_world;
+      let M : Model := ⟨
+          ⟨
+            Fin 3,
+            λ x y =>
+              match x, y with
+              | 0, 0 => True
+              | 0, 1 => True
+              | 1, 1 => True
+              | 1, 2 => True
+              | 2, 2 => True
+              | _, _ => False
+          ⟩,
+          λ w _ => w = 0 ∨ w = 1
+        ⟩;
+      use M, 0;
+      constructor;
+      . intro x;
+        match x with
+        | 0 => tauto;
+        | 1 => tauto;
+        | 2 => tauto;
+      . suffices (∀ (y : M.World), (0 : M.World) ≺ y → y = 0 ∨ y = 1) ∧ ∃ x, (0 : M.World) ≺ x ∧ ∃ y, x ≺ y ∧ y ≠ 0 ∧ y ≠ 1 by
+          simpa [M, Semantics.Realize, Satisfies];
+        constructor;
+        . intro y hy;
+          match y with
+          | 0 => tauto;
+          | 1 => tauto;
+          | 2 => tauto;
+        . use 1;
+          constructor;
+          . tauto;
+          . use 2;
+            refine ⟨by tauto, by trivial, by trivial⟩;
+
+theorem K4_ssubset_S4 : (Logic.K4) ⊂ (Logic.S4) := by
+  constructor;
+  . apply Hilbert.K4_weakerThan_S4;
+  . suffices ∃ φ, Hilbert.S4 ⊢! φ ∧ ¬TransitiveFrameClass ⊧ φ by simpa [K4.eq_TransitiveKripkeFrameClass_Logic];
+    use Axioms.T (.atom 0);
+    constructor;
+    . exact axiomT!;
+    . apply Formula.Kripke.ValidOnFrameClass.not_of_exists_model_world;
+      use ⟨⟨Fin 3, λ _ y => y = 1⟩, (λ w _ => w = 1)⟩, 0;
+      constructor;
+      . simp [Transitive];
+      . simp [Semantics.Realize, Satisfies];
+
+theorem K4_ssubset_GL : (Logic.K4) ⊂ (Logic.GL) := by
+  constructor;
+  . exact Hilbert.weakerThan_of_dominate_axioms $ by simp [axiomK!, axiomFour!];
+  . suffices ∃ φ, Hilbert.GL ⊢! φ ∧ ¬Hilbert.K4 ⊢! φ by simpa;
+    use (Axioms.L (.atom 0));
+    constructor;
+    . exact axiomL!;
+    . exact Hilbert.K4.unprovable_AxiomL;
+
+theorem S4_ssubset_Triv : (Logic.S4) ⊂ (Logic.Triv) := by
+  constructor;
+  . exact Hilbert.weakerThan_of_dominate_axioms $ by simp [axiomK!, axiomT!, axiomTc!];
+  . suffices ∃ φ, Hilbert.Triv ⊢! φ ∧ ¬ReflexiveTransitiveFrameClass ⊧ φ by simpa [S4.eq_ReflexiveTransitiveKripkeFrameClass_Logic];
+    use Axioms.Tc (.atom 0)
+    constructor;
+    . exact axiomTc!;
+    . apply Formula.Kripke.ValidOnFrameClass.not_of_exists_model_world;
+      unfold Axioms.Tc;
+      let M : Model := ⟨⟨Fin 2, λ x y => x ≤ y⟩, λ w _ => w = 0⟩;
+      use M, 0;
+      constructor;
+      . constructor;
+        . simp [M, Reflexive];
+        . unfold Transitive;
+          omega;
+      . suffices ∃ x, (0 : M.World) ≺ x ∧ ¬x = 0 by
+          simpa [M, Semantics.Realize, Satisfies];
+        use 1;
+        constructor;
+        . omega;
+        . trivial;
 
 end Logic
 
