Foundation/Modal/Hilbert/Geach.lean
@@ -20,6 +20,12 @@ lemma KTB.eq_Geach : Hilbert.KTB = Hilbert.Geach {⟨0, 0, 1, 0⟩, ⟨0, 1, 0, 
 
 lemma KT4B.eq_Geach : Hilbert.KT4B = Hilbert.Geach {⟨0, 0, 1, 0⟩, ⟨0, 2, 1, 0⟩, ⟨0, 1, 0, 1⟩} := by aesop;
 
+lemma K4.eq_Geach : Hilbert.K4 = Hilbert.Geach {⟨0, 2, 1, 0⟩} := by aesop;
+
+lemma KD.eq_Geach : Hilbert.KD = Hilbert.Geach {⟨0, 0, 1, 1⟩} := by aesop;
+
+lemma KDB.eq_Geach : Hilbert.KDB = Hilbert.Geach {⟨0, 0, 1, 1⟩, ⟨0, 1, 0, 1⟩} := by aesop;
+
 lemma S4.eq_Geach : Hilbert.S4 = Hilbert.Geach {⟨0, 0, 1, 0⟩, ⟨0, 2, 1, 0⟩} := by aesop;
 
 lemma S4Dot2.eq_Geach : Hilbert.S4Dot2 = Hilbert.Geach {⟨0, 0, 1, 0⟩, ⟨0, 2, 1, 0⟩, ⟨1, 1, 1, 1⟩} := by aesop;
