Foundation/Modal/Kripke/Hilbert/K4.lean
@@ -1,0 +1,54 @@
+import Foundation.Modal.Kripke.Hilbert.Geach
+import Foundation.Modal.Kripke.Filteration
+import Foundation.Modal.Kripke.FiniteFrame
+
+namespace LO.Modal
+
+open Kripke
+open Geachean
+
+abbrev Kripke.TransitiveFrameClass : FrameClass := { F | Transitive F }
+abbrev Kripke.TransitiveFiniteFrameClass : FiniteFrameClass := { F | Transitive F.Rel }
+
+namespace Hilbert.K4
+
+instance Kripke.sound : Sound (Hilbert.K4) (Kripke.TransitiveFrameClass) := by
+  convert Hilbert.Geach.Kripke.sound (G := {⟨0, 2, 1, 0⟩});
+  exact eq_Geach;
+  . unfold TransitiveFrameClass MultiGeacheanConfluentFrameClass MultiGeachean;
+    simp [Geachean.reflexive_def, Geachean.transitive_def];
+
+instance Kripke.consistent : System.Consistent (Hilbert.K4) := by
+  convert Hilbert.Geach.Kripke.Consistent (G := {⟨0, 2, 1, 0⟩});
+  exact eq_Geach;
+
+instance Kripke.complete : Complete (Hilbert.K4) (Kripke.TransitiveFrameClass) := by
+  convert Hilbert.Geach.Kripke.Complete (G := {⟨0, 2, 1, 0⟩});
+  . exact eq_Geach;
+  . unfold TransitiveFrameClass MultiGeacheanConfluentFrameClass MultiGeachean;
+    simp [Geachean.reflexive_def, Geachean.transitive_def];
+
+open finestFilterationTransitiveClosureModel in
+instance Kripke.finiteComplete : Complete (Hilbert.K4) (TransitiveFiniteFrameClass) := ⟨by
+  intro φ hp;
+  apply Kripke.complete.complete;
+  intro F F_trans V x;
+  let M : Kripke.Model := ⟨F, V⟩;
+  let FM := finestFilterationTransitiveClosureModel M φ.subformulas;
+  apply @filteration M φ.subformulas _ FM ?filterOf x φ (by simp) |>.mpr;
+  apply hp (by
+    suffices Finite (FilterEqvQuotient M φ.subformulas) by
+      simp only [FiniteFrameClass.toFrameClass];
+      use ⟨FM.toFrame⟩;
+      refine ⟨?_, rfl⟩;
+      . exact transitive;
+    apply FilterEqvQuotient.finite;
+    simp;
+  ) FM.Val;
+  . apply finestFilterationTransitiveClosureModel.filterOf;
+    exact F_trans;
+⟩
+
+end Hilbert.K4
+
+end LO.Modal
