Foundation/Modal/Kripke/Hilbert/Triv.lean
@@ -21,19 +21,29 @@ lemma Kripke.eq_EqualityFrameClass_ReflexiveCoreflexiveFrameClass : EqualityFram
 
 namespace Hilbert.Triv
 
-instance Kripke.Consistent : System.Consistent (Hilbert.Triv) := by
+instance Kripke.soundReflCorefl : Sound (Hilbert.Triv) (Kripke.ReflexiveCoreflexiveFrameClass) := by
+  convert Hilbert.Geach.Kripke.sound (G := {⟨0, 0, 1, 0⟩, ⟨0, 1, 0, 0⟩});
+  exact eq_Geach;
+  . unfold ReflexiveCoreflexiveFrameClass MultiGeacheanConfluentFrameClass MultiGeachean;
+    simp [Geachean.reflexive_def, Geachean.coreflexive_def];
+
+instance Kripke.soundEquality : Sound (Hilbert.Triv) (Kripke.EqualityFrameClass) := by
+  rw [eq_EqualityFrameClass_ReflexiveCoreflexiveFrameClass];
+  exact Kripke.soundReflCorefl;
+
+instance Kripke.consistent : System.Consistent (Hilbert.Triv) := by
   convert Hilbert.Geach.Kripke.Consistent (G := {⟨0, 0, 1, 0⟩, ⟨0, 1, 0, 0⟩});
   exact eq_Geach;
 
-instance Kripke.CompleteReflCorefl : Complete (Hilbert.Triv) (Kripke.ReflexiveCoreflexiveFrameClass) := by
+instance Kripke.completeReflCorefl : Complete (Hilbert.Triv) (Kripke.ReflexiveCoreflexiveFrameClass) := by
   convert Hilbert.Geach.Kripke.Complete (G := {⟨0, 0, 1, 0⟩, ⟨0, 1, 0, 0⟩});
   . exact eq_Geach;
   . unfold ReflexiveCoreflexiveFrameClass MultiGeacheanConfluentFrameClass MultiGeachean;
     simp [Geachean.reflexive_def, Geachean.coreflexive_def];
 
-instance Kripke.CompleteEquality : Complete (Hilbert.Triv) (Kripke.EqualityFrameClass) := by
+instance Kripke.completeEquality : Complete (Hilbert.Triv) (Kripke.EqualityFrameClass) := by
   rw [eq_EqualityFrameClass_ReflexiveCoreflexiveFrameClass];
-  exact Kripke.CompleteReflCorefl;
+  exact Kripke.completeReflCorefl;
 
 end Hilbert.Triv
 
